Session.v
@@ -21,8 +21,7 @@ Inductive protoExp : type -> protoType -> Type :=
 | ChoiceC (b:bool) {r s:protoType} {R S:type} :(protoExp R r) -> (protoExp S s)
     -> (protoExp (if(b) then R else S) (Choice r s))
 | OfferC {r s : protoType} {R S:type} : (protoExp R r) -> (protoExp S s)
-    -> (protoExp (Either R S) (Offer r s))  
-| ReturnC {t:type} : (message t) -> protoExp t (Eps t).
+                                        -> (protoExp (Either R S) (Offer r s))| ReturnC {t:type} : (message t) -> protoExp t (Eps t).
 
 Notation "x :!: y" := (Send x y)
                         (at level 50, left associativity). 
@@ -47,7 +46,7 @@ Notation "x :&: y" := (protoExp (Offer x y))
 Notation "'send' n ; p" := (SendC n p)
                             (right associativity, at level 60).
 Notation "x <- 'receive' ; p " := (ReceiveC (fun x => p)) 
-                                    (right associativity, at level 60). 
+                                    (right associativity, at level 60).
 
 Notation "'offer'" := OfferC.
 
@@ -64,8 +63,8 @@ Definition unwrapBasic (m:message Basic) : nat :=
   end.
 
 
-Definition enc1 := encrypt Basic (basic 42) (public 1). Check enc1.
-Definition enc2 := encrypt _ enc1 (public 2).
+Definition enc1 := encrypt (basic 42) (public 1). Check enc1.
+Definition enc2 := encrypt enc1 (public 2).
 Eval compute in decryptM enc1 (private 1).
 Eval compute in decryptM enc1 (private 0).
 Eval compute in decryptM enc2 (private 2).
@@ -90,11 +89,11 @@ Definition pairFst{t1 t2: type} (m:message (Pair t1 t2)) : message t1 :=
   | _ => bad _                
   end.
 
-Definition pair1 := pair _ _ (basic 1) (basic 2).
+Definition pair1 := pair (basic 1) (basic 2).
 Eval compute in pairFst pair1.
-Definition pair1' := pair _ _ (bad Basic) (basic 2).
+Definition pair1' := pair (bad Basic) (basic 2).
 Eval compute in pairFst pair1'.
-Definition pair1'' := pair _ _ (basic 1) (bad Basic).
+Definition pair1'' := pair  (basic 1) (bad Basic).
 Eval compute in pairFst pair1''.
 
 Definition pairSnd{t1 t2: type} (m:message (Pair t1 t2)) : message t2 :=
@@ -104,23 +103,33 @@ Definition pairSnd{t1 t2: type} (m:message (Pair t1 t2)) : message t2 :=
   | _ => bad _                
   end.
 
-Definition pair2 := pair _ _ (basic 1) (basic 2).
+Definition pair2 := pair (basic 1) (basic 2).
 Eval compute in pairSnd pair2.
-Definition pair2' := pair _ _ (basic 1) (bad Basic).
+Definition pair2' := pair (basic 1) (bad Basic).
 Eval compute in pairSnd pair2'.
 
-Fixpoint protoTypeLength (t:protoType) : nat :=
+(*Fixpoint protoTypeLength (t:protoType) : nat :=
   match t with
   | Send _ t' => 1 + (protoTypeLength t')
   | Receive _ t' => 1 + (protoTypeLength t')
-  | Choice p1 p2 => 1 + protoTypeLength p2
-  | Offer p1 p2 => 1 + protoTypeLength p2
+  | Choice p1 p2 => 1 + protoTypeLength p1
+  | Offer p1 p2 => 1 + protoTypeLength p1
   | Eps _ => 1                               
-  end.
+  end. *)
 
-Definition protoLength {t:protoType} {T:type} (p1:protoExp T t) : nat := protoTypeLength t.
+Fixpoint protoExpLength {T:type} {pt:protoType} (p: protoExp T pt) : nat :=
+  match p with
+  | SendC _ _ _ _ p' => 1 + (protoExpLength p')
+  | ReceiveC t _ _ f => 1 + (protoExpLength (f (bad t)))
+  | ChoiceC b _ _ _ _ p' p'' => if b then (protoExpLength p')
+                               else (protoExpLength p'')
+  | OfferC _ _ _ _ p' p'' => max (protoExpLength p') (protoExpLength p'')
+  | ReturnC _ _ => 1
+  end.                                                                                   
 
-Eval compute in protoTypeLength (Send Basic (Eps Basic)).
+Definition protoLength {t:protoType} {T:type} (p1:protoExp T t) : nat := (*protoTypeLength t*) protoExpLength p1.
+
+(*Eval compute in protoTypeLength (Send Basic (Eps Basic)). *)
 
 Fixpoint DualT' (t t':protoType) : Prop :=
   match t with
@@ -184,46 +193,75 @@ Proof.
   
 Defined.
 
-Definition Dual {t t':protoType} {T T':type} (p1:protoExp T t) (p2:protoExp T' t') : Prop := DualT t t'.            
+Definition Dual {t t':protoType} {T T':type} (p1:protoExp T t) (p2:protoExp T' t') : Prop := DualT t t'.           
 
 
-Fixpoint runProto' {t t':protoType} {T T':type} (p1:protoExp T t) (p2:protoExp T' t') (l: nat)
+Fixpoint runProto'' {t t':protoType} {T T':type} (p1:protoExp T t) (p2:protoExp T' t') (l: nat)
   : (message T) + {(~ (Dual p1 p2))}.
-Proof.
+Proof. destruct l. left. exact (bad T).
   case_eq p1; case_eq p2; intros;
+       
   (* Eliminate all un-interesting cases (20 of the 25 subgoals!) *)
   try (right; unfold not; intros; contradiction).
 
   (* Send/Receive case *)
-  destruct (eq_type_dec t0 t2). subst. clear H. clear H0. assert (message T1 + {~ Dual p0 (p m)}). apply (runProto' p'0 p' T1 T0 p0 (p m) (protoTypeLength p'0)). destruct X; try (right; unfold not; intros HH; inversion HH; contradiction). apply inleft. exact m0. right. unfold not. intros HH. inversion HH. symmetry in H1. contradiction.
+  destruct (eq_type_dec t0 t2). subst. clear H. clear H0. assert (message T1 + {~ Dual p0 (p m)}). apply (runProto'' p'0 p' T1 T0 p0 (p m) l(*(protoExpLength (p m))*)). destruct X; try (right; unfold not; intros HH; inversion HH; contradiction). apply inleft. exact m0. right. unfold not. intros HH. inversion HH. symmetry in H1. contradiction.
 
   (* Receive/Send case *)
-  destruct (eq_type_dec t0 t2). subst. clear H. clear H0. assert (message T1 + {~ Dual (p0 m) p }). apply (runProto' _ _ _ _ (p0 m) p (protoTypeLength p'0)). destruct X; try (right; unfold not; intros HH; inversion HH; contradiction). apply inleft. exact m0. right. unfold not. intros HH. inversion HH. symmetry in H1. contradiction.
+  destruct (eq_type_dec t0 t2). subst. clear H. clear H0. assert (message T1 + {~ Dual (p0 m) p }). apply (runProto'' _ _ _ _ (p0 m) p (*(protoExpLength (p0 m))*) l). destruct X; try (right; unfold not; intros HH; inversion HH; contradiction). apply inleft. exact m0. right. unfold not. intros HH. inversion HH. symmetry in H1. contradiction.
 
   (* Choice/Offer case *)
   destruct b; destruct (DualT_dec r0 r); destruct (DualT_dec s0 s).
 
     (* true case *)
-    clear H.  clear H0. destruct (runProto' _ _ _ _ p3 p (protoTypeLength r0)); try (right; unfold not; intros; destruct H1; contradiction). left. exact m. unfold not in n. unfold Dual in n. apply n in d. inversion d. right. unfold not. intros. destruct H1. contradiction. right. unfold not. intros. destruct H1. contradiction. right. unfold not. intros. destruct H1. contradiction.
+    clear H.  clear H0. destruct (runProto'' _ _ _ _ p3 p (*(protoExpLength p3)*) l); try (right; unfold not; intros; destruct H1; contradiction). left. exact m. unfold not in n. unfold Dual in n. apply n in d. inversion d. right. unfold not. intros. destruct H1. contradiction. right. unfold not. intros. destruct H1. contradiction. right. unfold not. intros. destruct H1. contradiction.
 
     (* false case *)
-    clear H.  clear H0. destruct (runProto' _ _ _ _ p4 p0 (protoTypeLength s0)); try (right; unfold not; intros; destruct H1; contradiction). left. exact m. unfold not in n. unfold Dual in n. apply n in d0. inversion d0. right. unfold not. intros. destruct H1. contradiction. right. unfold not. intros. destruct H1. contradiction. right. unfold not. intros. destruct H1. contradiction.
+    clear H.  clear H0. destruct (runProto'' _ _ _ _ p4 p0 (*(protoExpLength p4)*) l); try (right; unfold not; intros; destruct H1; contradiction). left. exact m. unfold not in n. unfold Dual in n. apply n in d0. inversion d0. right. unfold not. intros. destruct H1. contradiction. right. unfold not. intros. destruct H1. contradiction. right. unfold not. intros. destruct H1. contradiction.
 
   (* Offer/Choice case *)
   destruct b; destruct (DualT_dec r0 r); destruct (DualT_dec s0 s).
 
     (* true case *)
-    clear H.  clear H0. destruct (runProto' _ _ _ _ p3 p (protoTypeLength r0)); try (right; unfold not; intros; destruct H1; contradiction). left. exact (leither _ _ m). unfold not in n. unfold Dual in n. apply n in d. inversion d. right. unfold not. intros. destruct H1. contradiction. right. unfold not. intros. destruct H1. contradiction. right. unfold not. intros. destruct H1. contradiction.
+    clear H.  clear H0. destruct (runProto'' _ _ _ _ p3 p (*(protoExpLength p3)*) l); try (right; unfold not; intros; destruct H1; contradiction). left. exact (leither _ _ m). unfold not in n. unfold Dual in n. apply n in d. inversion d. right. unfold not. intros. destruct H1. contradiction. right. unfold not. intros. destruct H1. contradiction. right. unfold not. intros. destruct H1. contradiction.
 
     (* false case *)
-    clear H.  clear H0. destruct (runProto' _ _ _ _ p4 p0 (protoTypeLength s0)); try (right; unfold not; intros; destruct H1; contradiction). left. exact (reither _ _  m). unfold not in n. unfold Dual in n. apply n in d0. inversion d0. right. unfold not. intros. destruct H1. contradiction. right. unfold not. intros. destruct H1. contradiction. right. unfold not. intros. destruct H1. contradiction.
+    clear H.  clear H0. destruct (runProto'' _ _ _ _ p4 p0 (*(protoExpLength p4)*) l); try (right; unfold not; intros; destruct H1; contradiction). left. exact (reither _ _  m). unfold not in n. unfold Dual in n. apply n in d0. inversion d0. right. unfold not. intros. destruct H1. contradiction. right. unfold not. intros. destruct H1. contradiction. right. unfold not. intros. destruct H1. contradiction.
 
   (* Return case *)
-  left. exact m0. Defined.
+    left. exact m0.
+
+   
+Defined.
 
   
-Definition runProto {t t':protoType} {T T':type} (p1:protoExp T t) (p2:protoExp T' t')
-  : (message T) + {(~ (Dual p1 p2))} := runProto' p1 p2 (max (protoLength p1) (protoLength p2)).
+Definition runProto' {t t':protoType} {T T':type} (p1:protoExp T t) (p2:protoExp T' t')
+  : (message T) + {(~ (Dual p1 p2))} := runProto'' p1 p2 (1 + (max (protoLength p1) (protoLength p2))).
+
+Fixpoint DualTSymm {t t':protoType} : DualT t t' -> DualT t' t.
+Proof.
+  intros. destruct t; destruct t'; try (inversion H); try (
+  split;
+  subst; trivial;
+  apply (DualTSymm); assumption). Defined.
+
+Hint Resolve DualTSymm.
+
+Lemma notDualSymm {t t':protoType} {T T':type} {p1:protoExp T t} {p2:protoExp T' t'} : (~ Dual p1 p2) -> (~ Dual p2 p1).
+Proof. 
+  intros. unfold not. intros. apply DualTSymm in H0. unfold Dual in H. contradiction. Qed.
+
+  
+Definition runProto {t t':protoType} {T T':type} (p1:protoExp T t) (p2:protoExp T' t') : ((message T * message T') + {~ (Dual p1 p2)}).
+  refine(
+  match (runProto' p1 p2) with
+  | inleft m =>
+    match (runProto' p2 p1) with
+    | inleft m' => inleft (m, m')
+    | inright p => inright (notDualSymm p)
+    end
+  | inright p => inright p           
+  end). Defined.
 
 Definition proto3 :=
   send (basic 42);
@@ -255,8 +293,7 @@ Check proto5.
 
 Example dual45 : Dual proto4 proto5. unfold Dual. simpl. auto. Qed.
 
-Eval compute in (runProto proto5 proto4).
-Eval compute in (runProto proto4 proto5).
+Eval compute in runProto proto4 proto5.
 
 Definition proto6 (b:bool) :=
   choice b EpsC
@@ -280,31 +317,71 @@ Definition bPub := (public 2).
 Definition aPubBad := (public 3).
 Definition bPubBad := (public 4).
 Definition aPri := (private 1).
-Definition aPriBad := (private 5).
 Definition bPri := (private 2).
+Definition aPriBad := (private 5).
+Definition bPriBad := (private 6).
 
-Definition Needham_A :=
-  send (encrypt Basic (basic 1) bPub);
-  x <- receive;
-  (*y <- decrypt x using aPri; *)
-  send (encrypt _ (pairSnd (t1:=Basic) (t2:=Basic)
-                  (decryptM x aPri)) bPub);
-  ReturnC ((pairSnd (t1:=Basic) (t2:=Basic)
-                  (decryptM x aPri))). Check Needham_A.
+Definition Needham_A (myPri theirPub:keyType) :=
+  send (encrypt (basic 1) theirPub);
+  x <- receive; (* x : Encrypt (Pair Basic Basic) *) 
+  let y := decryptM x myPri in (* y : Pair Basic Basic *) 
+  let y' := (pairSnd (t1:=Basic) (t2:=Basic) y) in 
+  send (encrypt y' theirPub);
+  ReturnC (t:= (Pair Basic Basic)) y. Check Needham_A.
 
-Definition Needham_B :=
-  x <- receive;
-  (*y <- decrypt x using bPri; *)
-  send (encrypt _ (pair Basic Basic (decryptM x bPri) (basic 2)) aPub);
-  z <- receive;
-  ReturnC (t:= Pair Basic (Encrypt Basic)) (pair _ _ (decryptM x bPri) z). Check Needham_B.
+Definition Needham_B (myPri theirPub:keyType) :=
+  x <- receive; (* x : Encrypt Basic *)
+  let y := decryptM x myPri in (* y : Basic *)
+  send (encrypt (pair y (basic 2)) theirPub);
+  z <- receive; (* z : Encrypt Basic *)
+  let z' := decryptM z myPri in    (* z' : Basic *)
+  ReturnC (t:= Pair Basic (Basic)) (pair y z'). Check Needham_B.
 
-Example DualNeedham : Dual Needham_A Needham_B.
+
+
+Example DualNeedham {a b c d:keyType} : Dual (Needham_A a b) (Needham_B c d).
 Proof. unfold Dual; simpl. repeat( split;trivial). Qed.
 
-Eval compute in runProto Needham_A Needham_B.
-Eval compute in runProto Needham_B Needham_A.
+Definition Needham_A_good := (Needham_A aPri bPub).
+Definition Needham_B_good := (Needham_B bPri aPub).
+
+Eval compute in runProto Needham_A_good Needham_B_good.
+
+Definition Needham_A_badAuth := (Needham_A aPriBad bPub).
+Definition Needham_A_badEncrypt := (Needham_A aPri bPubBad).
+Definition Needham_B_badAuth := (Needham_B bPriBad aPub).
+Definition Needham_B_badEncrypt := (Needham_B bPri aPubBad).
+
+Eval compute in runProto Needham_A_good Needham_B_badAuth.
+Eval compute in runProto Needham_A_good Needham_B_badEncrypt.
+
+Eval compute in runProto Needham_B_good Needham_A_badAuth.
+Eval compute in runProto Needham_B_good Needham_A_badEncrypt.
+
+Eval compute in runProto Needham_A_badAuth Needham_B_badAuth.
+Eval compute in runProto Needham_A_badAuth Needham_B_badEncrypt.
+
+Eval compute in runProto Needham_A_badEncrypt Needham_B_badAuth.
+Eval compute in runProto Needham_A_badEncrypt Needham_B_badEncrypt.
+
+Definition protoAuth1 (theirPub:keyType) :=
+  let m1 := encrypt (basic 1) theirPub in
+  send m1;
+  x <- receive;
+  ReturnC (t:=Basic) x. Check protoAuth1.
+
+Definition protoAuth2 (myPri:keyType) :=
+  x <- receive;
+  let m1 := decryptM x myPri in
+  send m1;
+  ReturnC (t:=Basic) m1. Check protoAuth2.
+
+Definition protoAuthGoodResult :=  runProto (protoAuth1 (public 2)) (protoAuth2 (private 2)). Eval compute in protoAuthGoodResult.
+
+Example uniqueAuth : forall k,
+    (runProto (protoAuth1 (public 2)) (protoAuth2 k)) = protoAuthGoodResult
+    -> (k = (private 2)).
+Proof.
+  intros. destruct protoAuthGoodResult. inversion H. destruct (eq_key_dec k (private 2)). assumption. Abort.
        
-
-
 End session.
